code/ecdsap256/Hacl.Impl.P256.MixedPointAdd.fst
@@ -30,6 +30,10 @@ open FStar.Mul
 friend Hacl.Impl.P256.PointAdd
 
 
+open Hacl.Impl.P256.Q.Comparision
+open Hacl.Impl.P256.Q.PrimitivesMasking
+
+
 #set-options "--z3rlimit 300 --fuel 0 --ifuel 0"
 
 inline_for_extraction noextract 
@@ -46,8 +50,13 @@ val pointAffineIsNotZero: p: pointAffine -> Stack uint64
 let pointAffineIsNotZero p = 
   let x = sub p (size 0) (size 4) in 
   let y = sub p (size 4) (size 4) in 
-  let xZero = isZero_uint64_CT_global x in 
-  let yZero = isZero_uint64_CT_global y in 
+
+(*   let xZero = isZero_uint64_CT_global x in 
+  let yZero = isZero_uint64_CT_global y in  *)
+
+  let xZero = eq_felem_0_u64 #Private (global_to_comparable x) in 
+  let yZero = eq_felem_0_u64 #Private (global_to_comparable y) in 
+
   logand_lemma xZero yZero;
   logand xZero yZero
 
@@ -146,7 +155,7 @@ let computeZ3_point_add_mixed z3 z1 h tempBuffer =
   montgomery_multiplication_buffer_by_one z1 z1z2;
   montgomery_multiplication_buffer z1z2 h z3
 
-inline_for_extraction noextract
+(* inline_for_extraction noextract
 val cmovznz: out: felem -> x: felem -> y: felem -> mask: uint64 -> Stack unit
   (requires fun h -> as_nat h x < prime256 /\ as_nat h y < prime256 /\
     live h out /\ live h x /\ live h y /\ (uint_v mask == 0 \/ uint_v mask = pow2 64 - 1))
@@ -182,7 +191,7 @@ let cmovznz out x y mask =
   cmovznz4_lemma mask (Seq.index y 1) (Seq.index x 1);
   cmovznz4_lemma mask (Seq.index y 2) (Seq.index x 2);
   cmovznz4_lemma mask (Seq.index y 3) (Seq.index x 3)
-
+ *)
 
 inline_for_extraction noextract
 val cmovznz_one_mm: out: felem -> mask: uint64 -> Stack unit
@@ -276,7 +285,8 @@ let copy_point_conditional_affine_to_result out q maskPoint =
   let h0 = ST.get() in 
   
   let pZ = sub maskPoint (size 8) (size 4) in 
-  let mask = isZero_uint64_CT pZ in 
+  (* let mask = isZero_uint64_CT pZ in  *)
+  let mask = eq_felem_0_u64 #Private pZ in 
 
   let xOut = sub out (size 0) (size 4) in 
   let yOut = sub out (size 4) (size 4) in 
@@ -409,9 +419,9 @@ let copy_point_conditional result x p maskPoint =
   let result_y = sub result (size 4) (size 4) in 
   let result_z = sub result (size 8) (size 4) in 
 
-  cmovznz4 mask x_x p_x result_x;
-  cmovznz4 mask x_y p_y result_y;
-  cmovznz4 mask x_z p_z result_z;
+  cmovznz4 p_x x_x result_x mask;
+  cmovznz4 p_y x_y  result_y mask;
+  cmovznz4 p_z x_z  result_z mask;
 
   let mX = as_nat_il h0 (gsub maskPoint (size 0) (size 4)) in 
   let mY = as_nat_il h0 (gsub maskPoint (size 4) (size 4)) in 
