code/ecdsap256/Hacl.Impl.P256.LowLevel.PrimeSpecific.fst
@@ -18,6 +18,8 @@ open FStar.Math.Lemmas
 open FStar.Mul
 open Lib.IntTypes.Intrinsics
 
+open Hacl.Impl.P256.Q.PrimitivesMasking
+
 #reset-options " --z3rlimit 300"
 
 
@@ -48,7 +50,7 @@ let reduction_prime256_2prime256_with_carry_impl cin x result =
       assert(uint_v c <= 1);
       assert(if uint_v c = 0 then as_nat h0 x >= prime256 else as_nat h0 x < prime256);
     let carry = sub_borrow_u64 c cin (u64 0) tempBufferForSubborrow in 
-    cmovznz4 carry tempBuffer x result;
+    cmovznz4 result tempBuffer x carry;
   let h1 = ST.get() in 
       assert_norm (pow2 64 * pow2 64 * pow2 64 * pow2 64 = pow2 256);
       assert_norm (prime256 < pow2 256);
@@ -86,7 +88,7 @@ let reduction_prime256_2prime256_8_with_carry_impl x result =
       recall_contents prime256_buffer (Lib.Sequence.of_list p256_prime_list); 
     let c = Hacl.Impl.P256.LowLevel .sub4_il x_ prime256_buffer tempBuffer in 
     let carry = sub_borrow_u64 c cin (u64 0) tempBufferForSubborrow in 
-    cmovznz4 carry tempBuffer x_ result; 
+    cmovznz4 result tempBuffer x_ carry; 
       let h4 = ST.get() in 
       assert_norm (pow2 256 > prime256);
       assert(if (wide_as_nat h0 x < prime256) then begin
@@ -132,7 +134,7 @@ let reduction_prime_2prime_impl x result =
     recall_contents prime256_buffer (Lib.Sequence.of_list p256_prime_list);
         let h0 = ST.get() in 
     let c = sub4_il x prime256_buffer tempBuffer in 
-    cmovznz4 c tempBuffer x result;
+    cmovznz4 result tempBuffer x c;
       let h2 = ST.get() in 
     lemma_reduction1 (as_nat h0 x) (as_nat h2 result);
   pop_frame()  
