code/ecdsap256/Hacl.Impl.P256.LowLevel.RawCmp.fst
@@ -14,7 +14,6 @@ inline_for_extraction noextract
 val eq_u8_nCT: a:uint8 -> b:uint8 -> (r:bool{r == (uint_v a = uint_v b)})
 
 let eq_u8_nCT a b =
-  let open Lib.RawIntTypes in
   FStar.UInt8.(u8_to_UInt8 a =^ u8_to_UInt8 b)
 
 
@@ -22,7 +21,6 @@ inline_for_extraction noextract
 val eq_u64_nCT: a:uint64 -> b:uint64 -> (r:bool{r == (uint_v a = uint_v b)})
 
 let eq_u64_nCT a b =
-  let open Lib.RawIntTypes in
   FStar.UInt64.(u64_to_UInt64 a =^ u64_to_UInt64 b)
 
 
