code/ecdsap256/Hacl.Impl.P256.Q.Comparision.fst
@@ -1,0 +1,166 @@
+module Hacl.Impl.P256.Q.Comparision
+
+open FStar.HyperStack.All
+open FStar.HyperStack
+module ST = FStar.HyperStack.ST
+
+open Lib.IntTypes
+open Lib.Buffer
+
+open Spec.P256.Definitions
+
+
+
+#set-options " --z3rlimit 100"
+
+type qualification = 
+  |Public
+  |Private
+
+let invert_qualif (a: qualification): Lemma
+  (requires True) 
+  (ensures (inversion qualification))
+  [SMTPat (qualification)] =
+  allow_inversion (qualification) 
+
+
+inline_for_extraction noextract
+val unsafe_bool_of_u64 (x: uint64 { v x == 0 \/ v x == pow2 64 - 1 }):
+  (b:bool { b <==> v x == 0 })
+
+let unsafe_bool_of_u64 x = 
+  let open Lib.RawIntTypes in
+  FStar.UInt64.(u64_to_UInt64 x =^ 0uL)
+
+
+val eq_u64_u64_u64: #q: qualification -> a: uint64 -> b: uint64 -> Tot uint64
+
+let eq_u64_u64_u64 #q a b = 
+  match q with 
+  |Public -> begin
+      let open Lib.RawIntTypes in
+      let r = FStar.UInt64.(u64_to_UInt64 a =^ u64_to_UInt64 b) in 
+      match r with 
+      |true -> u64 0
+      |false -> u64 (maxint U64) end
+  |Private -> 
+    eq_mask_lemma a b;
+    eq_mask a b
+
+
+val eq_u64_u64_bool: #q: qualification -> a: uint64 -> b: uint64 -> Tot bool
+
+let eq_u64_u64_bool #q a b = 
+  match q with 
+  |Public -> 
+    let open Lib.RawIntTypes in 
+    FStar.UInt64.(u64_to_UInt64 a =^ u64_to_UInt64 b) 
+  |Private -> 
+    eq_mask_lemma a b;
+    let r = eq_mask a b in 
+    unsafe_bool_of_u64 r
+
+
+val neq_u64_u64_u64: #q: qualification -> a: uint64 -> b: uint64 -> Tot uint64
+
+let neq_u64_u64_u64 #q a b = 
+  lognot_lemma (eq_u64_u64_u64 #q a b);
+  lognot (eq_u64_u64_u64 #q a b)
+
+
+val eq_u64_0_u64: #q: qualification -> a: uint64 -> Tot uint64
+
+let eq_u64_0_u64 #q a = 
+  eq_u64_u64_u64 #q a (u64 0) 
+
+
+val neq_u64_0_u64: #q: qualification -> a: uint64 -> Tot uint64
+
+let neq_u64_0_u64 #q a = 
+  neq_u64_u64_u64 #q a (u64 0)
+
+
+
+inline_for_extraction noextract
+val eq_felem_0_u64: #q: qualification -> #buf_type: buftype -> f: lbuffer_t buf_type uint64 (size 4) -> Stack uint64
+  (requires fun h -> live h f)
+  (ensures fun h0 r h1 -> modifies0 h0 h1 /\ 
+  (if as_nat h0 f = 0 then uint_v r == pow2 64 - 1 else uint_v r == 0))
+
+
+let eq_felem_0_u64 #q f = 
+  let a0 = index f (size 0) in 
+  let a1 = index f (size 1) in 
+  let a2 = index f (size 2) in 
+  let a3 = index f (size 3) in 
+
+  let r0 = eq_u64_0_u64 #q a0 in 
+  let r1 = eq_u64_0_u64 #q a1 in 
+  let r2 = eq_u64_0_u64 #q a2 in 
+  let r3 = eq_u64_0_u64 #q a3 in 
+
+  let r01 = logand r0 r1 in 
+  let r23 = logand r2 r3 in 
+  let r = logand r01 r23 in 
+
+  logand_lemma r0 r1; 
+  logand_lemma r2 r3;
+  logand_lemma r01 r23;
+  r
+
+
+val global_to_comparable: glbuffer uint64 (size 4) -> Stack (lbuffer_t IMMUT uint64 (size 4))
+  (requires fun h -> True)
+  (ensures fun h0 _ h1 -> True)
+
+let global_to_comparable f = (const_to_ilbuffer f) <: lbuffer_t IMMUT uint64 (size 4)
+
+
+val cmp_felem_felem_u64: #q:qualification -> #buf_type0: buftype -> #buf_type1: buftype -> 
+  a: lbuffer_t buf_type0 uint64 (size 4) -> b: lbuffer_t buf_type1 uint64 (size 4) -> Stack uint64
+  (requires fun h -> True)
+  (ensures fun h0 _ h1 -> True)
+
+
+let cmp_felem_felem_u64 #q #b0 #b1 a b = 
+  let a_0 = index a (size 0) in 
+  let a_1 = index a (size 1) in 
+  let a_2 = index a (size 2) in 
+  let a_3 = index a (size 3) in 
+
+  let b_0 = index b (size 0) in 
+  let b_1 = index b (size 1) in 
+  let b_2 = index b (size 2) in 
+  let b_3 = index b (size 3) in 
+
+  let r_0 = eq_u64_u64_u64 #q a_0 b_0 in 
+  let r_1 = eq_u64_u64_u64 #q a_1 b_1 in
+  let r_2 = eq_u64_u64_u64 #q a_2 b_2 in 
+  let r_3 = eq_u64_u64_u64 #q a_3 b_3 in 
+
+  let r01 = logand r_0 r_1 in 
+  let r23 = logand r_2 r_3 in 
+  let r = logand r01 r23 in 
+  
+  logand_lemma r_0 r_1;
+  logand_lemma r_2 r_3;
+  logand_lemma r01 r23;
+  
+  eq_mask_lemma a_0 b_0;
+  eq_mask_lemma a_1 b_1;
+  eq_mask_lemma a_2 b_2;
+  eq_mask_lemma a_3 b_3;
+  (* lemma_equality (a_0, a_1, a_2, a_3) (b_0, b_1, b_2, b_3); *)
+  r
+
+
+val cmp_felem_felem_bool: #q:qualification -> #buf_type0: buftype -> #buf_type1: buftype -> 
+  a: lbuffer_t buf_type0 uint64 (size 4) -> b: lbuffer_t buf_type1 uint64 (size 4) -> Stack bool
+  (requires fun h -> True)
+  (ensures fun h0 _ h1 -> True)
+
+
+let cmp_felem_felem_bool #q #b0 #b1 a b = 
+  admit();
+  let f = cmp_felem_felem_u64 #q #b0 #b1 a b in 
+  unsafe_bool_of_u64 f
