code/ecdsap256/Hacl.Impl.P256.Q.PrimitivesMasking.fst
@@ -5,107 +5,13 @@ open FStar.HyperStack
 module ST = FStar.HyperStack.ST
 
 open Lib.IntTypes
-open Hacl.Impl.P256.Arithmetics
 
 open Lib.Buffer
-open Hacl.Impl.P256.LowLevel
 
 open Spec.P256.Definitions
 open Spec.P256.Lemmas
 
 
-
-inline_for_extraction noextract
-val cmovznz01: a: uint64 -> b: uint64 -> mask: uint64 {uint_v mask = 0 \/ uint_v mask = 1} -> 
-  Tot (r: uint64 {if uint_v mask = 0 then uint_v r = uint_v a else uint_v r = uint_v b})
-
-let cmovznz01 a b mask = 
-  let mask = (u64 0) -. mask in 
-  lemma_xor_copy_cond a b mask;
-  logxor a (logand mask (logxor a b))
-
-
-inline_for_extraction noextract
-val cmovznz: a: uint64 -> b: uint64 -> mask: uint64 {uint_v mask = 0 \/ uint_v mask = pow2 64 - 1} -> 
-  Tot (r: uint64 {if uint_v mask = 0 then uint_v r = uint_v a else uint_v r = uint_v b})
-
-let cmovznz a b mask = 
-  lemma_xor_copy_cond a b mask;
-  logxor a (logand mask (logxor a b))
-
-
-
-val cmovznz4: out: felem -> x: felem -> y: felem -> mask: uint64 -> Stack unit
-  (requires fun h -> live h out /\ live h x /\ live h y /\ (uint_v mask == 0 \/ uint_v mask = pow2 64 - 1))
-  (ensures fun h0 _ h1 -> modifies (loc out) h0 h1 /\ (
-    if v mask = 0
-      then as_nat h1 out == as_nat h0 x
-      else 
-	as_nat h1 out == as_nat h0 y))
-
-let cmovznz4 out x y mask = 
-  let h0 = ST.get() in 
-  
-  let out_0 = index out (size 0) in 
-  let out_1 = index out (size 1) in 
-  let out_2 = index out (size 2) in 
-  let out_3 = index out (size 3) in  
-
-  let mask = eq_mask mask (u64 0) in 
-  
-  let r0 = logor (logand x.(size 0) mask) (logand y.(size 0) (lognot mask)) in 
-  let r1 = logor (logand x.(size 1) mask) (logand y.(size 1) (lognot mask)) in 
-  let r2 = logor (logand x.(size 2) mask) (logand y.(size 2) (lognot mask)) in 
-  let r3 = logor (logand x.(size 3) mask) (logand y.(size 3) (lognot mask)) in 
-
-  upd out (size 0) r0;
-  upd out (size 1) r1;
-  upd out (size 2) r2;
-  upd out (size 3) r3;
-
-  let x = as_seq h0 x in 
-  let y = as_seq h0 y in 
-  cmovznz4_lemma mask (Seq.index y 0) (Seq.index x 0);
-  cmovznz4_lemma mask (Seq.index y 1) (Seq.index x 1);
-  cmovznz4_lemma mask (Seq.index y 2) (Seq.index x 2);
-  cmovznz4_lemma mask (Seq.index y 3) (Seq.index x 3)
-
-
-
-
-val cswap8:  x: widefelem -> y: widefelem -> mask: uint64 -> Stack unit 
-  (requires fun h -> True)
-  (ensures fun h0 _ h1 -> True)
-
-let cswap8 p1 p2 bit = 
-  let open Lib.Sequence in 
-  let h0 = ST.get () in
-  let mask = bit in
-
-  [@ inline_let]
-  let inv h1 (i:nat{i <= 8}) = 
-    (forall (k:nat{k < i}).
-      if v bit = 1
-      then (as_seq h1 p1).[k] == (as_seq h0 p2).[k] /\ (as_seq h1 p2).[k] == (as_seq h0 p1).[k]
-      else (as_seq h1 p1).[k] == (as_seq h0 p1).[k] /\ (as_seq h1 p2).[k] == (as_seq h0 p2).[k]) /\
-    (forall (k:nat{i <= k /\ k < 12}).
-      (as_seq h1 p1).[k] == (as_seq h0 p1).[k] /\ (as_seq h1 p2).[k] == (as_seq h0 p2).[k]) /\
-    modifies (loc p1 |+| loc p2) h0 h1 in
- 
-  Lib.Loops.for 0ul 8ul inv
-    (fun i ->
-      let dummy = mask &. (p1.(i) ^. p2.(i)) in
-      p1.(i) <- p1.(i) ^. dummy;
-      p2.(i) <- p2.(i) ^. dummy;
-      lemma_cswap2_step bit ((as_seq h0 p1).[v i]) ((as_seq h0 p2).[v i])
-    );
-  let h1 = ST.get () in
-  Lib.Sequence.eq_intro (as_seq h1 p1) (if v bit = 1 then as_seq h0 p2 else as_seq h0 p1);
-  Lib.Sequence.eq_intro (as_seq h1 p2) (if v bit = 1 then as_seq h0 p1 else as_seq h0 p2)
-
-
-    
-  
 
 inline_for_extraction noextract
 val copy_conditional: out: felem -> x: felem -> mask: uint64{uint_v mask = 0 \/ uint_v mask = pow2 64 - 1} -> Stack unit 
@@ -145,3 +51,90 @@ let copy_conditional out x mask =
 
   lemma_eq_funct_ (as_seq h1 out) (as_seq h0 out);
   lemma_eq_funct_ (as_seq h1 out) (as_seq h0 x)
+
+
+val cmovznz4: out: felem -> x: felem -> y: felem -> mask: uint64 -> Stack unit
+  (requires fun h -> live h out /\ live h x /\ live h y /\ (uint_v mask == 0 \/ uint_v mask = pow2 64 - 1))
+  (ensures fun h0 _ h1 -> modifies (loc out) h0 h1 /\ (
+    if v mask = 0 then as_nat h1 out == as_nat h0 x else as_nat h1 out == as_nat h0 y))
+
+let cmovznz4 out x y mask = 
+  let h0 = ST.get() in 
+  
+  let out_0 = index out (size 0) in 
+  let out_1 = index out (size 1) in 
+  let out_2 = index out (size 2) in 
+  let out_3 = index out (size 3) in  
+
+  let mask = eq_mask mask (u64 0) in 
+  
+  let r0 = logor (logand x.(size 0) mask) (logand y.(size 0) (lognot mask)) in 
+  let r1 = logor (logand x.(size 1) mask) (logand y.(size 1) (lognot mask)) in 
+  let r2 = logor (logand x.(size 2) mask) (logand y.(size 2) (lognot mask)) in 
+  let r3 = logor (logand x.(size 3) mask) (logand y.(size 3) (lognot mask)) in 
+
+  upd out (size 0) r0;
+  upd out (size 1) r1;
+  upd out (size 2) r2;
+  upd out (size 3) r3;
+
+  let x = as_seq h0 x in 
+  let y = as_seq h0 y in 
+  cmovznz4_lemma mask (Seq.index y 0) (Seq.index x 0);
+  cmovznz4_lemma mask (Seq.index y 1) (Seq.index x 1);
+  cmovznz4_lemma mask (Seq.index y 2) (Seq.index x 2);
+  cmovznz4_lemma mask (Seq.index y 3) (Seq.index x 3)
+
+
+
+
+inline_for_extraction noextract
+val cmovznz01: a: uint64 -> b: uint64 -> mask: uint64 {uint_v mask = 0 \/ uint_v mask = 1} -> 
+  Tot (r: uint64 {if uint_v mask = 0 then uint_v r = uint_v a else uint_v r = uint_v b})
+
+let cmovznz01 a b mask = 
+  let mask = (u64 0) -. mask in 
+  lemma_xor_copy_cond a b mask;
+  logxor a (logand mask (logxor a b))
+
+
+inline_for_extraction noextract
+val cmovznz: a: uint64 -> b: uint64 -> mask: uint64 {uint_v mask = 0 \/ uint_v mask = pow2 64 - 1} -> 
+  Tot (r: uint64 {if uint_v mask = 0 then uint_v r = uint_v a else uint_v r = uint_v b})
+
+let cmovznz a b mask = 
+  lemma_xor_copy_cond a b mask;
+  logxor a (logand mask (logxor a b))
+
+
+
+
+val cswap8:  x: widefelem -> y: widefelem -> mask: uint64 -> Stack unit 
+  (requires fun h -> True)
+  (ensures fun h0 _ h1 -> True)
+
+let cswap8 p1 p2 bit = 
+  let open Lib.Sequence in 
+  let h0 = ST.get () in
+  let mask = bit in
+
+  [@ inline_let]
+  let inv h1 (i:nat{i <= 8}) = 
+    (forall (k:nat{k < i}).
+      if v bit = 1
+      then (as_seq h1 p1).[k] == (as_seq h0 p2).[k] /\ (as_seq h1 p2).[k] == (as_seq h0 p1).[k]
+      else (as_seq h1 p1).[k] == (as_seq h0 p1).[k] /\ (as_seq h1 p2).[k] == (as_seq h0 p2).[k]) /\
+    (forall (k:nat{i <= k /\ k < 12}).
+      (as_seq h1 p1).[k] == (as_seq h0 p1).[k] /\ (as_seq h1 p2).[k] == (as_seq h0 p2).[k]) /\
+    modifies (loc p1 |+| loc p2) h0 h1 in
+ 
+  Lib.Loops.for 0ul 8ul inv
+    (fun i ->
+      let dummy = mask &. (p1.(i) ^. p2.(i)) in
+      p1.(i) <- p1.(i) ^. dummy;
+      p2.(i) <- p2.(i) ^. dummy;
+      lemma_cswap2_step bit ((as_seq h0 p1).[v i]) ((as_seq h0 p2).[v i])
+    );
+  let h1 = ST.get () in
+  Lib.Sequence.eq_intro (as_seq h1 p1) (if v bit = 1 then as_seq h0 p2 else as_seq h0 p1);
+  Lib.Sequence.eq_intro (as_seq h1 p2) (if v bit = 1 then as_seq h0 p1 else as_seq h0 p2)
